wip

src/Std/Data/DTreeMap/Slice.lean
@@ -47,7 +47,7 @@ public instance : Iterator (RxcIterator α β cmp) Id ((a : α) × β a) where
           out (by simpa using h))
       else
         pure (.done (by simpa using h))
-    | ⟨⟨map, none, bound, pf⟩⟩ => .done rfl
+    | ⟨⟨map, none, bound, pf⟩⟩ => pure (.done rfl)
 
 public instance : IteratorCollect (RxcIterator α β cmp) Id Id := .defaultImplementation
 
@@ -111,6 +111,45 @@ def instFinitenessRelation [TransCmp cmp] : FinitenessRelation (RxcIterator α �
 public instance instFinite [TransCmp cmp] : Finite (RxcIterator α β cmp) Id :=
   .of_finitenessRelation instFinitenessRelation
 
+public theorem step_rxcIterator_eq_match {α β} {cmp : α → α → Ordering} [TransCmp cmp] {it : IterM (α := RxcIterator α β cmp) Id _} :
+    it.step = pure (match h : it.internalState.next with
+      | some next =>
+        if h' : (cmp next.fst it.internalState.bound).isLE then
+          .yield ⟨it.internalState.treeMap, it.internalState.treeMap.getEntryGT? next.fst, it.internalState.bound, (by apply getEntryGE?_getEntryGT?_eq_some)⟩ next
+            (by simp [IterM.IsPlausibleStep, Iterator.IsPlausibleStep, h', h])
+        else
+          .done (by simpa [IterM.IsPlausibleStep, Iterator.IsPlausibleStep, h] using h')
+      | none =>
+        .done (by simp [IterM.IsPlausibleStep, Iterator.IsPlausibleStep, h])) := by
+  simp [IterM.step, Iterator.step]
+  split
+  · simp
+    split <;> simp
+  · simp
+
+private theorem Option.filter_eq_none_iff_all {α} {o : Option α} {p : α → Bool} :
+    o.filter p = none ↔ o.all (! p ·) := by
+  simp [Option.all_eq_true]
+
+public theorem step_rxcIterator_eq_match' {α β} {cmp : α → α → Ordering} [TransCmp cmp] {it : IterM (α := RxcIterator α β cmp) Id _} :
+    it.step = pure (match h : it.internalState.next.filter (fun e => (cmp e.fst it.internalState.bound).isLE) with
+      | some next =>
+        .yield ⟨it.internalState.treeMap, it.internalState.treeMap.getEntryGT? next.fst, it.internalState.bound, (by apply getEntryGE?_getEntryGT?_eq_some)⟩ next
+          (by simpa [IterM.IsPlausibleStep, Iterator.IsPlausibleStep, and_comm (a := (_ = true))] using h)
+      | none =>
+        haveI : ∀ e, it.internalState.next = some e → cmp e.fst it.internalState.bound = .gt := by
+          simpa using h
+        .done (by simpa only [IterM.IsPlausibleStep, Iterator.IsPlausibleStep, Option.filter_eq_none_iff_all,
+            Ordering.not_isLE_eq_isGT, ← Ordering.isGT_iff_eq_gt, Bool.decide_eq_true] using h)) := by
+  rw [step_rxcIterator_eq_match]
+  sorry
+
+-- public theorem RxcIterator.induct {α β} {cmp : α → α → Ordering} [TransCmp cmp]
+--     (motive : Iter (α := RxcIterator α β cmp) _ → Sort x)
+--     (step : (it : Iter (α := RxcIterator α β cmp) _) →
+--         (ih_yield : ))
+--     {it : Iter (α := RxcIterator α β cmp) _}
+
 end Rxc
 
 public structure RccSliceData (α : Type u) (β : α → Type v)
@@ -123,40 +162,199 @@ public abbrev RccSlice α β cmp := Slice (RccSliceData α β cmp)
 public instance : Rcc.Sliceable (DTreeMap α β cmp) α (RccSlice α β cmp) where
   mkSlice carrier range := ⟨carrier, range⟩
 
+@[always_inline]
+public def RccSlice.Internal.iterM (s : RccSlice α β cmp) : IterM (α := RxcIterator α β cmp) Id ((a : α) × β a) :=
+  ⟨⟨s.1.treeMap, s.1.treeMap.getEntryGE? s.1.range.lower, s.1.range.upper,
+      by apply getEntryGE?_getEntryGE?_eq_some⟩⟩
+
 public instance {s : RccSlice α β cmp} : ToIterator s Id ((a : α) × β a) where
   State := RxcIterator α β cmp
-  iterMInternal := ⟨⟨s.1.treeMap, s.1.treeMap.getEntryGE? s.1.range.lower, s.1.range.upper,
-      by apply DTreeMap.getEntryGE?_getEntryGE?_eq_some⟩⟩
+  /-
+  There is a good reason to extract the iterator into a separate function `RccSlice.Internal.iterM`:
+  The `Iterator` instance on `ToIterator.State` needs to unfold `ToIterator.State`, which requires
+  unfolding this `ToIterator` instance. In consequence, the definition of `iterMInternal` is also
+  unfolded. Because it is complex and highly dependent, this is not desirable.
+  See `Std.Iterators.instIteratorState`.
+  -/
+  iterMInternal := RccSlice.Internal.iterM s
 
 #eval (.ofList [⟨0, 0⟩, ⟨1, 1⟩, ⟨100, 3⟩, ⟨101, 4⟩] : DTreeMap Nat (fun _ => Nat) compare)[2...=102].toList
 
 public theorem step_iter_rccSlice_eq_match {α β} {cmp : α → α → Ordering} [TransCmp cmp] {t : DTreeMap α β cmp} {a b : α} :
-    t[a...=b].iter.step = (match t.getEntryGE? a with
-      | _ => sorry) := by
-  sorry
-
-public theorem step_iter_rccSlice_eq_match {α β} {cmp : α → α → Ordering} [TransCmp cmp] {t : DTreeMap α β cmp} {a b : α} :
-    t[a...=b].iter.step = (match t.getEntryGE? a with
+    t[a...=b].iter.step = (match h : t.getEntryGE? a with
       | some next =>
-        if (cmp next b).isLE then
-          .yield sorry sorry sorry
+        if h' : (cmp next.fst b).isLE then
+          .yield ⟨t, t.getEntryGT? next.fst, b, (by apply getEntryGE?_getEntryGT?_eq_some)⟩ next
+            (by simp [Iter.IsPlausibleStep, IterM.IsPlausibleStep, Iterator.IsPlausibleStep, Slice.iter_eq_toIteratorIter, ToIterator.iter_eq, RccSlice.Internal.iterM, Rcc.Sliceable.mkSlice, Iter.toIterM, IterM.toIter, h', h])
         else
-          .done sorry
+          .done (by simpa [Iter.IsPlausibleStep, IterM.IsPlausibleStep, Iterator.IsPlausibleStep, Slice.iter_eq_toIteratorIter, ToIterator.iter_eq, RccSlice.Internal.iterM, Rcc.Sliceable.mkSlice, h] using h')
       | none =>
-        .done sorry) := by
-  sorry
+        .done (by simp [Iter.IsPlausibleStep, IterM.IsPlausibleStep, Iterator.IsPlausibleStep, Slice.iter_eq_toIteratorIter, ToIterator.iter_eq, RccSlice.Internal.iterM, Rcc.Sliceable.mkSlice, h])) := by
+  simp only [Iter.step, PlausibleIterStep.yield, PlausibleIterStep.done]
+  rw [step_rxcIterator_eq_match]
+  simp only [PlausibleIterStep.yield, PlausibleIterStep.done, Id.run_pure]
+  simp only [RccSlice.Internal.iterM, Iter.toIterM, Slice.iter_eq_toIteratorIter, ToIterator.iter_eq, IterM.toIter]
+  simp [Rcc.Sliceable.mkSlice]
+  split <;> rename_i heq
+  · simp only [Slice.iter_eq_toIteratorIter, ToIterator.iter_eq, IterM.toIter, RccSlice.Internal.iterM] at heq
+    split <;> split <;> simp_all [IterM.toIter]
+  · simp only [Slice.iter_eq_toIteratorIter, ToIterator.iter_eq, IterM.toIter, RccSlice.Internal.iterM] at heq
+    split <;> simp_all
 
-theorem rccSlice_toList_eq_map_rcc_toList {α β} {cmp : α → α → Ordering} [TransCmp cmp] {t : DTreeMap α β cmp} {a b : α} :
-    t[a...=b].toList = (a...=b).toList
-      := by
-  sorry
+public theorem val_step_iter_rccSlice_eq_match {α β} {cmp : α → α → Ordering} [TransCmp cmp] {t : DTreeMap α β cmp} {a b : α} :
+    t[a...=b].iter.step.val = (match t.getEntryGE? a with
+      | some next =>
+        if (cmp next.fst b).isLE then
+          .yield ⟨t, t.getEntryGT? next.fst, b, (by apply getEntryGE?_getEntryGT?_eq_some)⟩ next
+        else
+          .done
+      | none =>
+        .done) := by
+  rw [step_iter_rccSlice_eq_match]
+  split <;> split <;> simp_all
+
+public theorem val_step_iter_rccSlice_eq_match' {α β} {cmp : α → α → Ordering} [TransCmp cmp] {t : DTreeMap α β cmp} {a b : α} :
+    t[a...=b].iter.step.val = (match (t.getEntryGE? a).filter (fun e => (cmp e.fst b).isLE) with
+      | some next =>
+        .yield ⟨t, t.getEntryGT? next.fst, b, (by apply getEntryGE?_getEntryGT?_eq_some)⟩ next
+      | none =>
+        .done) := by
+  rw [val_step_iter_rccSlice_eq_match]
+  split
+  · split <;> simp_all [Option.filter_some]
+  · simp_all
+
+theorem toList_rccSlice_eq_toList_rccSlice {α β} {cmp : α → α → Ordering} [TransCmp cmp] {t t': DTreeMap α β cmp} {a b a' b' : α}
+    (h : ∀ c, (c ∈ t.toList ∧ (cmp a c.fst).isLE ∧ (cmp c.fst b).isLE) ↔ (c ∈ t'.toList ∧ (cmp a' c.fst).isLE ∧ (cmp c.fst b').isLE)) :
+    t[a...=b].toList = t'[a'...=b'].toList := by
+    -- simp only [Slice.toList_eq_toList_iter, Slice.iter_eq_toIteratorIter, ToIterator.iter_eq,
+    --   RccSlice.Internal.iterM, Rcc.Sliceable.mkSlice, IterM.toIter]
+    simp only [Slice.toList_eq_toList_iter]
+    induction hi : Slice.iter (Rcc.Sliceable.mkSlice t a...=b) using Iter.inductSteps
+    rw [← hi]
+    rw [Iter.toList_eq_match_step, Iter.toList_eq_match_step]
+    simp only [val_step_iter_rccSlice_eq_match']
+    have : (t.getEntryGE? a).filter (fun e => (cmp e.fst b).isLE) =
+        (t'.getEntryGE? a').filter (fun e => (cmp e.fst b').isLE) := by
+      ext e
+      simp [getEntryGE?_eq_some_iff]
+      specialize h
+      constructor
+      · intro h'
+        have he := (h e).mp ⟨h'.1.1, h'.1.2.1, h'.2⟩
+        refine ⟨⟨he.1, he.2.1, ?_⟩, he.2.2⟩
+        intro k hk hk'
+        by_cases hkb : (cmp k b').isLE
+        · simp only [← map_fst_toList_eq_keys, List.mem_map] at hk
+          obtain ⟨f, hfm, rfl⟩ := hk
+          have hf := (h f).mpr ⟨hfm, hk', hkb⟩
+          apply h'.1.2.2
+          · simpa only [← map_fst_toList_eq_keys] using List.mem_map_of_mem hf.1
+          · exact hf.2.1
+        · refine TransCmp.isLE_trans he.2.2 ?_
+          apply Ordering.isLE_of_eq_lt
+          simpa [OrientedCmp.gt_iff_lt] using hkb
+      · intro h'
+        have he := (h e).mpr ⟨h'.1.1, h'.1.2.1, h'.2⟩
+        refine ⟨⟨he.1, he.2.1, ?_⟩, he.2.2⟩
+        intro k hk hk'
+        by_cases hkb : (cmp k b).isLE
+        · simp only [← map_fst_toList_eq_keys, List.mem_map] at hk
+          obtain ⟨f, hfm, rfl⟩ := hk
+          have hf := (h f).mp ⟨hfm, hk', hkb⟩
+          apply h'.1.2.2
+          · simpa only [← map_fst_toList_eq_keys] using List.mem_map_of_mem hf.1
+          · exact hf.2.1
+        · refine TransCmp.isLE_trans he.2.2 ?_
+          apply Ordering.isLE_of_eq_lt
+          simpa [OrientedCmp.gt_iff_lt] using hkb
+    simp [this]
+    cases Option.filter (fun e => (cmp e.fst b').isLE) (t'.getEntryGE? a')
+    · simp
+    · simp
+
+    match hn : t.getEntryGE? a, hn' : t'.getEntryGE? a' with
+    | none, none => simp
+    | some next, some next' =>
+      have heq : ∀ e, (e ∈ t.toList ∧ (cmp a e.fst).isLE ∧ ∀ k, k ∈ t.keys → (cmp a k).isLE → (cmp e.fst k).isLE) →
+          e = next := by simp [← getEntryGE?_eq_some_iff, hn, Option.some_inj]
+      simp [getEntryGE?_eq_some_iff] at hn hn'
+      have hm : next.fst ∈ t.keys := by simpa only [← map_fst_toList_eq_keys] using List.mem_map_of_mem hn.1
+      have hm' : next'.fst ∈ t'.keys := by simpa only [← map_fst_toList_eq_keys] using List.mem_map_of_mem hn'.1
+      have hle : (cmp next.fst b).isLE → (cmp next'.fst next.fst).isLE := by
+        intro h'
+        have := (h next).mp ⟨hn.1, hn.2.1, h'⟩
+        exact hn'.2.2 next.fst
+          (by simpa only [← map_fst_toList_eq_keys] using List.mem_map_of_mem this.1)
+          this.2.1
+      have hle' : (cmp next'.fst b').isLE → (cmp next.fst next'.fst).isLE := by
+        intro h'
+        have := (h next').mpr ⟨hn'.1, hn'.2.1, h'⟩
+        exact hn.2.2 next'.fst
+          (by simpa only [← map_fst_toList_eq_keys] using List.mem_map_of_mem this.1)
+          this.2.1
+      have : (cmp next.fst b).isLE ↔ (cmp next'.fst b').isLE := by
+        constructor
+        · intro h'
+          have := (h next).mp ⟨hn.1, hn.2.1, h'⟩
+          exact TransCmp.isLE_trans (hle h') this.2.2
+        · intro h'
+          have := (h next').mpr ⟨hn'.1, hn'.2.1, h'⟩
+          exact TransCmp.isLE_trans (hle' h') this.2.2
+      by_cases h' : (cmp next.fst b).isLE
+      · have : next' = next := by
+          apply heq
+          have h'' := this.mp h'
+          have := (h next').mpr ⟨hn'.1, hn'.2.1, h''⟩
+          refine ⟨this.1, this.2.1, ?_⟩
+          intro k hk hk'
+          exact TransCmp.isLE_trans (hle h') (hn.2.2 k hk hk')
+        cases this
+        simp [h', this.mp h']
+      · have : ¬ (cmp next'.fst b').isLE := by simpa [this] using h'
+        simp [h', this]
+    | none, some x =>
+      sorry
+    | some x, none =>
+      sorry
+
 theorem rccSlice_toList_eq_filter_toList {α β} {cmp : α → α → Ordering} [TransCmp cmp] {t : DTreeMap α β cmp} {a b : α} :
     t[a...=b].toList = t.toList.filter (fun e => (cmp a e.fst).isLE ∧ (cmp e.fst b).isLE)
       := by
-  induction h : t.toList.length
-  · rw [length_toList, ← beq_iff_eq, ← isEmpty_eq_size_eq_zero] at h
-    simp [Slice.toList_eq_toList_iter, Slice.iter_eq_toIteratorIter, ToIterator.iter, ToIterator.iterM, ToIterator.iterMInternal]
-    rw [DTreeMap.toList_eq_nil]
-    simp? [length_toList, ← beq_iff_eq, ← isEmpty_eq_size_eq_zero] at h
+  let n := t.size
+  have hn : t.size ≤ n := by exact Nat.le_refl _
+  clear_value n
+  induction n generalizing t
+  · simp only [length_toList, Nat.le_zero_eq] at hn
+    rw [← beq_iff_eq, ← isEmpty_eq_size_eq_zero, ← isEmpty_toList] at hn
+    -- non-confluence: List.isEmpty_iff, DTreeMap.isEmpty_toList applied to t.toList.isEmpty
+    simp only [List.isEmpty_iff] at hn
+    simp only [Slice.toList_eq_toList_iter]
+    rw [Iter.toList_eq_match_step]
+    simp only [val_step_iter_rccSlice_eq_match]
+    cases h' : t.getEntryGE? a
+    · simp [hn]
+    · simp [getEntryGE?_eq_some_iff, hn] at h'
+  · rename_i n ih
+    by_cases hn : t.size = n + 1; rotate_left
+    · exact ih (by omega)
+    simp [Slice.toList_eq_toList_iter]
+    rw [Iter.toList_eq_match_step]
+    simp [val_step_iter_rccSlice_eq_match]
+    match h : t.getEntryGE? a with
+    | some next =>
+      simp [getEntryGE?_eq_some_iff] at h
+      let t' := t.erase next.fst
+      have : t'.size ≤ n := by
+        simp only [t', size_erase, ← mem_iff_contains, mem_of_mem_toList h.1, ↓reduceIte]
+        omega
+      specialize ih this
+      simp only [Slice.toList_eq_toList_iter, Slice.iter_eq_toIteratorIter, ToIterator.iter_eq,
+        RccSlice.Internal.iterM, Rcc.Sliceable.mkSlice, IterM.toIter] at ih
+      by_cases h' : (cmp next.fst b).isLE
+      · simp [h']
+
+    | none => simp
+
 
 end Std.DTreeMap
